Definition of vprop using tprop
+ tprop: vprop indexed by its type to allow a bind notation
+ a tactic to derive the interpretation lemmas of a tprop

steel/Learn.Steel.DLList.Data.fst
@@ -4,6 +4,7 @@ module U   = Learn.Util
 module T   = FStar.Tactics
 module TL  = Learn.Tactics.Logic
 module US  = Learn.Steel.Util
+module TP  = Learn.Steel.TProp
 module Mem = Steel.Memory
 
 #set-options "--fuel 1 --ifuel 1"
@@ -11,211 +12,61 @@ module Mem = Steel.Memory
 
 (**** Definition of the vprop *)
 
-let rec dllist0 (p : list_param) (entry : ref p.r) (len : nat) (exit : ref p.r)
-  : Pure vprop (requires True) (ensures fun v -> t_of v == dllist_sel_t p entry len exit)
-               (decreases len)
-  =
+let rec dllist_tp (p : list_param) (entry : ref p.r) (len : nat) (exit : ref p.r)
+  : Tot (TP.tprop (dllist_sel_t p entry len exit)) (decreases len)
+  = TP.(
     if len = 0
-    then
-      vrewrite emp #(dllist_sel_t p entry len exit)
-        (fun _ -> dll_nil entry exit)
-    else
+    then return (dll_nil entry exit)
+    else begin
       let len' = len - 1 in
-      vrewrite (vcell p entry `vdep` (fun c ->
-          let entry' = (p.cell entry).get_ref c Forward in
-          dllist0 p entry' len' exit `vrefine` (fun sl1 ->
-            let sl1 : dllist_sel_t p entry' len' exit = U.cast _ sl1 in
-            sl1.dll_prv == entry)))
-        #(dllist_sel_t p entry len exit)
-        (fun (|c, sl1|) -> dll_cons #p #entry #((p.cell entry).get_ref c Forward) #len' #exit c sl1)
-
-
-(**** Expansion the vprop *)
+      c   <-- vprt (t_of (vcell p entry)) (vcell p entry); 
+      let entry' = (p.cell entry).get_ref c Forward in
+      sl1 <-- tpr (dllist_tp p entry' len' exit);
+      _   <-- tpure (sl1.dll_prv == entry);
+      return #(dllist_sel_t p entry len exit)
+             (dll_cons #p #entry #((p.cell entry).get_ref c Forward) #len' #exit c sl1)
+    end
+  )
 
 let dllist_sl (p : list_param) entry len exit =
-  let VUnit r = dllist0 p entry len exit in r.hp
+  (dllist_tp p entry len exit).t_hp
 
-let dllist_sel (p : list_param) (entry : ref p.r) (len : nat) (exit : ref p.r) =
-  let VUnit r = dllist0 p entry len exit in r.sel
-
-let dllist_eq0 (p : list_param) (entry : ref p.r) (len : nat) (exit : ref p.r)
-  : Lemma (dllist p entry len exit == dllist0 p entry len exit)
-          [SMTPat (dllist p entry len exit)]
-  = let VUnit _ = dllist0 p entry len exit in ()
+let dllist_sel (p : list_param) entry len exit =
+  (dllist_tp p entry len exit).t_sel
 
 
 (**** Intro/Elim lemmas *)
 
+let rew () = T.norm [delta_only [`%dllist_tp]; zeta]
+
 let dllist_nil_interp (p : list_param) (entry : ref p.r) (exit : ref p.r) (m : Mem.mem)
-  : squash (Mem.interp (hp_of (dllist0 p entry 0 exit)) m /\
-            sel_of (dllist0 p entry 0 exit) m == dll_nil entry exit)
   =
-    let g0 : squash (Mem.interp (hp_of emp) m)
-      = reveal_emp ();
-        Mem.intro_emp m
-    in
-    _ by T.(
-      norm [delta_only [`%dllist0]; zeta]; norm [iota; primops];
-      split ();
-        (norm [delta_only [`%hp_of]; zeta];
-        norm [delta_only [`%vrewrite; `%vrewrite'; `%Mkvprop'?.hp]; iota];
-        exact (``@g0));
-        (norm [delta_only [`%sel_of]; zeta];
-        norm [delta_only [`%vrewrite; `%vrewrite'; `%Mkvprop'?.sel]; iota];
-        apply_lemma (`vrewrite_sel_eq))
-  )
-
-// TODO:MOVE
-let rec process_hyps (ts : list (T.term -> T.Tac (list T.term))) (hs : list T.term) : T.Tac (list T.term)
-  = T.(match hs with
-    | [] -> []
-    | h0 :: hs -> try first (map (fun (t : term -> Tac (list term)) () ->
-                               let hs0 = t h0 in process_hyps ts (hs0 @ hs)) ts)
-                with | _ -> h0 :: process_hyps ts hs
-  )
-
-
-let interp_star' (p q: Mem.slprop) (m: Mem.mem)
-  : Lemma Mem.(interp (p `star` q) m <==>
-      (exists (mp: mem) (mq: mem) . (disjoint mp mq /\ join mp mq == m) /\ (interp p mp /\ interp q mq)))
-  = Mem.interp_star p q m
-
-let sel_disj_eq_r (m m0 m1 : Mem.mem) (h_m : squash (Mem.disjoint m0 m1 /\ Mem.join m0 m1 == m))
-                  (#a : Type) (hp : Mem.slprop) (s : selector a hp)
-  : Lemma (requires Mem.interp hp m1)
-          (ensures (Mem.join_commutative m0 m1; s m1 == s m))
-  = Mem.join_commutative m0 m1
-
-let dllist_cons_interp0 (p : list_param) (entry : ref p.r) (len : nat) (exit : ref p.r) (m : Mem.mem)
-  : squash (Mem.interp (hp_of (dllist0 p entry (len + 1) exit)) m
-         <==> Mem.interp (hp_of (vcell p entry)) m /\
-           (let c = sel_of (vcell p entry) m in
-            let entry' = (p.cell entry).get_ref c Forward in
-            Mem.interp (hp_of (vcell p entry) `Mem.star` hp_of (dllist0 p entry' len exit)) m /\
-           (let sl1 : dllist_sel_t p entry' len exit
-                    = sel_of (dllist0 p entry' len exit) m in
-            sl1.dll_prv == entry)))
-  =
-    let rew_len_neq_0 () : Lemma (len + 1 = 0 == false) = () in
-    _ by T.(
-      apply (`TL.rew_iff_left);
-        norm [delta_only [`%dllist0]; zeta]; norm [iota];
-        l_to_r [``@rew_len_neq_0];
-        norm [delta_only [`%hp_of; `%vrewrite; `%vrewrite'; `%vdep; `%vdep'; `%Mkvprop'?.hp]; iota; zeta];
-        apply_lemma (`interp_vdep_hp);
-      apply (`TL.conj_morph_iff); apply (`TL.iff_refl);
-      let _ = intro () in
-      apply (`TL.rew_iff_left ); apply_lemma (`interp_star');
-      apply (`TL.rew_iff_right); apply (`TL.conj_morph_iff);
-        apply_lemma (`interp_star'); let _ = intro () in apply (`TL.iff_refl);
-      apply (`TL.rew_iff_left);
-        apply (`TL.exists_morph_iff); let _ = intro () in
-        apply (`TL.exists_morph_iff); let _ = intro () in
-        apply (`TL.conj_morph_iff); apply (`TL.iff_refl);
-        let h_m = intro () in let h_m, _ = T.destruct_and h_m in
-        let rew_sl = pose (`sel_disj_eq_r _ _ _ (Squash.return_squash (`#h_m))) in
-        apply (`TL.conj_morph_iff); apply (`TL.iff_refl);
-        let _ = intro () in
-        apply (`TL.rew_iff_left);
-          norm [delta_only [`%hp_of; `%Mkvprop'?.hp]; zeta; iota];
-          apply_lemma (`interp_vrefine_hp);
-        apply (`TL.conj_morph_iff); apply (`TL.iff_refl);
-          let _ = intro () in
-          l_to_r [binder_to_term rew_sl];
-          apply (`TL.iff_refl); smt ();
-      norm [delta_only [`%vcell]];
-      smt ())
+    let tp = dllist_tp p entry 0 exit in
+    assert (Mem.interp (hp_of (dllist p entry 0 exit)) m /\
+            sel_of (dllist p entry 0 exit) m == dll_nil entry exit)
+      by T.(let _ = TP.pose_interp_lemma (`(`@tp)) (``@m) rew [1] in smt ())
 
 let dllist_cons_interp (p : list_param) (entry : ref p.r) (len : nat) (exit : ref p.r) (m : Mem.mem)
-  = dllist_cons_interp0 p entry len exit m
-
-
-unfold
-let ref_hmem (m : Mem.mem) (v : vprop)
-  : Pure (hmem v) (requires Mem.interp (hp_of v) m) (ensures fun m' -> m' == m)
-  = m
-
-let vrewrite_sel_eq'
-      (v: vprop) (#t: Type) (f: (normal (t_of v) -> GTot t)) (h: Mem.hmem (normal (hp_of v)))
-      (sl0 : t_of v) (sl0_eq : squash (sel_of v h == sl0))
-  : squash ((vrewrite_sel v f <: selector' _ _) h == f sl0)
-  = vrewrite_sel_eq v f h
-
-let vdep_sel_eq'
-      (v: vprop) (p: ( (t_of v) -> Tot vprop)) (m: Mem.hmem (vdep_hp v p))
-      (sl0 : t_of v) (sl0_eq : squash (Mem.interp (hp_of v) m) -> squash (sel_of v m == sl0))
-      (sl1 : t_of (p sl0)) (sl1_eq : squash (Mem.interp (hp_of (p sl0)) m) -> squash (sel_of (p sl0) m == sl1))
-  : squash (vdep_sel v p m == (|sl0, sl1|))
   =
-    interp_vdep_hp v p m;
-    sl0_eq ();
-    sl1_eq ();
-    vdep_sel_eq v p m
-
-let vrefine_sel_eq'_aux
-      (v: vprop) (p: (normal (t_of v) -> Tot prop)) (m: Mem.hmem (vrefine_hp v p))
-      (sl0 : t_of v) (sl0_eq : squash (Mem.interp (hp_of v) m) -> squash (sel_of v m == sl0))
-  : Lemma (p sl0)
-  = vrefine_sel_eq v p m;
-    sl0_eq ()
-
-let vrefine_t_eq_ty
-      (v: vprop) (p: (normal (t_of v) -> Tot prop))
-      (sl0 sl1 : vrefine_t v p)
-      (_ : squash (eq2 #(t_of v) sl0 sl1))
-  : squash (eq2 #(vrefine_t v p) sl0 sl1)
-  = ()
-
-let vrefine_sel_eq'
-      (v: vprop) (p: (normal (t_of v) -> Tot prop)) (m: Mem.hmem (vrefine_hp v p))
-      (sl0 : t_of v) (sl0_eq : squash (Mem.interp (hp_of v) m) -> squash (sel_of v m == sl0))
-  : squash (eq2 #(t_of v) (vrefine_sel v p m) sl0)
-  =
-    vrefine_sel_eq v p m;
-    sl0_eq ()
-
-
-let change_eq_type (#a #b : Type) (x y : a) (_ : squash (a == b)) (_ : squash (eq2 #b x y))
-  : squash (eq2 #a x y)
-  = ()
-
-let dllist_cons_sel_eq0
-      (p : list_param) (entry : ref p.r) (len : nat) (exit : ref p.r) (m : Mem.mem)
-      (_ : squash (Mem.interp (hp_of (dllist0 p entry (len + 1) exit )) m))
-  : squash (dllist_cons_interp0 p entry len exit m;
-            let c = sel_of (vcell p entry) (ref_hmem m (vcell p entry)) in
-            let entry' = (p.cell entry).get_ref c Forward               in
-            let sl1 = sel_of (dllist0 p entry' len exit) m              in
-            sel_of (dllist0 p entry (len + 1) exit) m
-              == dll_cons #p #entry #entry' #len #exit c sl1)
-  =
-    let _ = dllist_cons_interp0 p entry len exit m in
-    let rew_len_neq_0 () : Lemma (len + 1 = 0 == false) = () in
-    let rew_len_1     () : Lemma (len + 1 - 1 ==   len) = () in
-    _ by T.(
-      apply_lemma (`U.eq2_trans);
-      norm [delta_only [`%dllist0]; zeta]; norm [iota];
-      l_to_r [``@rew_len_neq_0];
-      norm [delta_only [`%sel_of; `%Mkvprop'?.sel; `%vrewrite; `%vrewrite']; iota; zeta];
-      apply (`vrewrite_sel_eq');
-      norm [delta_only [`%sel_of; `%Mkvprop'?.sel; `%vdep; `%vdep']; iota; zeta];
-      apply (`change_eq_type); later ();
-      apply (`vdep_sel_eq');
-      let _ = intro () in trefl ();
-      let _ = intro () in
-      norm [delta_only [`%sel_of; `%Mkvprop'?.sel; `%vrefine; `%vrefine']; iota; zeta];
-      norm [delta_only [`%t_of]; zeta];
-      norm [delta_only [`%Mkvprop'?.t]; iota];
-      apply (`vrefine_t_eq_ty); apply (`change_eq_type); later ();
-      apply (`vrefine_sel_eq');
-      let _ = intro () in trefl ();
-
-      norm [iota]; l_to_r [``@rew_len_1]; trefl ();
-      trefl ();
-      trefl ())
+    let tp = dllist_tp p entry (len + 1) exit in
+    assert (Mem.interp (hp_of (dllist p entry (len + 1) exit)) m
+         <==> Mem.interp (hp_of (vcell p entry)) m /\
+           (let c = sel_of (vcell p entry) m              in
+            let entry' = (p.cell entry).get_ref c Forward in
+            Mem.interp (hp_of (vcell p entry) `Mem.star` hp_of (dllist p entry' len exit)) m /\
+           (let sl1 : dllist_sel_t p entry' len exit
+                    = sel_of (dllist p entry' len exit) m in
+            sl1.dll_prv == entry)))
+      by T.(let _ = TP.pose_interp_lemma (`(`@tp)) (``@m) rew [2] in smt ())
 
 let dllist_cons_sel_eq
       (p : list_param) (entry : ref p.r) (len : nat) (exit : ref p.r) (m : Mem.mem)
-  = 
+  =
+    let tp = dllist_tp p entry (len + 1) exit in
     dllist_cons_interp p entry len exit m;
-    dllist_cons_sel_eq0 p entry len exit m ()
+    assert (let c      = sel_of (vcell p entry) m            in
+            let entry' = (p.cell entry).get_ref c Forward    in
+            let sl1    = sel_of (dllist p entry' len exit) m in
+            sel_of (dllist p entry (len + 1) exit) m
+              == dll_cons #p #entry #entry' #len #exit c sl1)
+      by T.(let _ = TP.pose_interp_lemma (`(`@tp)) (``@m) rew [2] in smt ())
