steel/Learn.Steel.TProp.Test.fst
@@ -1,0 +1,52 @@
+module Learn.Steel.TProp.Test
+
+module T = FStar.Tactics
+
+open Steel.Memory
+open Steel.Effect.Atomic
+open Steel.Reference
+open Learn.Steel.TProp
+
+let vptr_opt_tp (#a : Type) (rb : ghost_ref bool) (rx : ref a) : tprop (option a)
+  =
+    b <-- vpr (ghost_vptr rb);
+    if b
+    then begin
+      x <-- vprt a (vptr rx);
+      return (Some x)
+    end else
+      return None
+
+let vptr_opt (#a : Type) (rb : ghost_ref bool) (rx : ref a) : vprop
+  = vprop_of_tprop (vptr_opt_tp rb rx)
+
+let intro_vptr_opt_Some #a rb rx (m : mem)
+      (_ : squash (interp (hp_of (ghost_vptr rb `star` vptr rx)) m /\
+                   b2t (sel_of (ghost_vptr rb) m)))
+  : squash (interp (hp_of (vptr_opt rb rx)) m /\
+            sel_of (vptr_opt rb rx) m == Some (sel_of (vptr rx) m))
+  = _ by T.(
+    let _ =
+      pose_interp_lemma (`vptr_opt_tp (`@rb) (`@rx)) (``@m)
+        (fun () -> norm [delta_only [`%vptr_opt_tp]])
+        [1]
+    in smt ())
+
+let elim_vptr_opt #a (rb : ghost_ref bool) (rx : ref a) (m : mem)
+  : Lemma (requires interp (hp_of (vptr_opt rb rx)) m)
+          (ensures  interp (hp_of (ghost_vptr rb)) m /\
+                    (if coerce_eq _ (sel_of (ghost_vptr rb) m)
+                     then interp (hp_of (ghost_vptr rb `star` vptr rx)) m /\
+                          sel_of (vptr_opt rb rx) m == Some (sel_of (vptr rx) m)
+                     else sel_of (vptr_opt rb rx) m == None #a))
+  =
+    let tp  = vptr_opt_tp rb rx in
+    let rew () = T.norm [delta_only [`%vptr_opt_tp]] in
+    assert (interp (hp_of (ghost_vptr rb)) m)
+      by T.(let _ = pose_interp_lemma (`(`@tp)) (``@m) rew [0] in smt ());
+    if coerce_eq _ (sel_of (ghost_vptr rb) m)
+    then assert (interp (hp_of (ghost_vptr rb `star` vptr rx)) m /\
+                 sel_of (vptr_opt rb rx) m == Some (sel_of (vptr rx) m))
+           by T.(let _ = pose_interp_lemma (`(`@tp)) (``@m) rew [1] in smt ())
+    else assert (sel_of (vptr_opt rb rx) m == None #a)
+           by T.(let _ = pose_interp_lemma (`(`@tp)) (``@m) rew [2] in smt ())
