steel/Learn.Steel.TProp.fst
@@ -1,0 +1,272 @@
+module Learn.Steel.TProp
+
+#set-options "--fuel 1 --ifuel 1"
+
+let interp_of_opt (slp : option slprop) (m : mem)
+  = Mem.intro_emp m
+
+let star_of_opt (slp0 slp1 : option slprop)
+  = match slp0 with
+    | None      -> Mem.star_commutative Mem.emp (slprop_of_opt slp1); Mem.emp_unit (slprop_of_opt slp1)
+    | Some slp0 ->
+    match slp1 with
+    | None      -> Mem.emp_unit slp0
+    | Some slp1 -> ()
+
+let interp_star_opt (slp0 slp1 : option slprop) (m : mem)
+  = calc (<==>) {
+    interp_opt (star_opt slp0 slp1) m;
+  <==> { interp_of_opt (star_opt slp0 slp1) m;
+       star_of_opt slp0 slp1 }
+    interp (slprop_of_opt slp0 `Mem.star` slprop_of_opt slp1) m;
+  <==> { Mem.interp_star (slprop_of_opt slp0) (slprop_of_opt slp1) m }
+    exists (m0 m1 : mem) . disjoint m0 m1 /\ join m0 m1 == m /\
+                      interp (slprop_of_opt slp0) m0 /\ interp (slprop_of_opt slp1) m1;
+  <==> { FStar.Classical.forall_intro (interp_of_opt slp0);
+       FStar.Classical.forall_intro (interp_of_opt slp1) }
+    exists (m0 m1 : mem) . disjoint m0 m1 /\ join m0 m1 == m /\
+                      interp_opt slp0 m0 /\ interp_opt slp1 m1;
+  }
+
+
+let tprop_interp_intro
+      #t u guard req slp sel
+      (int_sl : (m : mem) -> squash (guard m) ->
+                squash (interp u.t_hp m <==> req m /\ interp_opt (slp m) m))
+      (sel_eq : (m : Mem.hmem u.t_hp) -> squash (guard m /\ req m /\ interp_opt (slp m) m) ->
+                squash (u.t_sel m == sel m))
+      (join0  : (m0:mem{guard m0 /\ req m0}) -> (m1:mem{disjoint m0 m1}) ->
+                   squash (let m = join m0 m1 in guard m /\ req m /\ slp m == slp m0 /\ sel m == sel m0))
+      (join1  : (m0:mem) -> (m1:mem{disjoint m0 m1}) ->
+                   squash (let m = join m0 m1 in guard m /\ req m /\ (interp u.t_hp m0 \/ interp_opt (slp m) m0)) ->
+                   squash (guard m0 /\ req m0))
+  : tprop_interp u guard req slp sel
+  = {
+    tpi_int_sl =
+      introduce forall (m : mem {guard m}) . (interp u.t_hp m <==> req m /\ interp_opt (slp m) m)
+        with int_sl m ();
+    tpi_sel_eq =
+      introduce forall (m : Mem.hmem u.t_hp {guard m /\ req m}) . u.t_sel m == sel m
+        with (int_sl m (); sel_eq m ());
+    tpi_join0 =
+      introduce forall (m0: mem{guard m0 /\ req m0}) (m1:mem{disjoint m0 m1}) .
+                guard (join m0 m1) /\ req (join m0 m1) /\ slp (join m0 m1) == slp m0 /\ sel (join m0 m1) == sel m0
+        with join0 m0 m1;
+    tpi_join1 =
+      introduce forall (m0:mem) (m1:mem{disjoint m0 m1}) .
+                (guard (join m0 m1) /\ req (join m0 m1) /\
+                  (interp u.t_hp m0 \/ interp_opt (slp (join m0 m1)) m0)) ==>
+                (guard m0 /\ req m0)
+        with introduce _ ==> _ with _ . join1 m0 m1 ();
+  }
+
+let tprop_interp_elim
+      #t #u #guard #req #slp #sel tpi
+      (m : mem)
+  = tpi.tpi_int_sl; tpi.tpi_sel_eq
+
+let tprop_interp_join0
+      #t (#u : tprop t) #guard #req #slp #sel (tpi : tprop_interp u guard req slp sel)
+      (m0 m1 : mem)
+  : Lemma (requires disjoint m0 m1 /\ guard m0)
+          (ensures (let m = join m0 m1 in
+                    req m0 ==> (guard m /\ req m /\ slp m == slp m0 /\ sel m == sel m0)))
+  = tpi.tpi_join0
+
+let tprop_interp_join1
+      #t (#u : tprop t) #guard #req #slp #sel (tpi : tprop_interp u guard req slp sel)
+      (m0 m1 : mem)
+  : Lemma (requires disjoint m0 m1)
+          (ensures  (guard (join m0 m1) /\ req (join m0 m1) /\
+                      (interp u.t_hp m0 \/ interp_opt (slp (join m0 m1)) m0)) ==>
+                    (guard m0 /\ req m0))
+  = tpi.tpi_join1
+
+
+let tprop_trivial_interp (#t : Type) (u : tprop t)
+  = tprop_interp_intro _ _ _ _ _
+      (fun m _ -> ()) (fun m _ -> ()) (fun m0 m1 -> ()) (fun m0 m1 _ -> ())
+
+let tprop_of_vprop_interp (t : Type) (v : vprop {normal (t_of v) == t})
+  = tprop_interp_intro _ _ _ _ _
+      (fun m _ -> ()) (fun m _ -> ()) (fun m0 m1 -> ()) (fun m0 m1 _ -> ())
+
+
+(***** [treturn] *)
+
+let treturn_sel (#a : Type) (x : erased a) : selector a Mem.emp
+  =
+    let sel' (_ : Mem.hmem Mem.emp) : GTot a = x in
+    sel'
+
+let treturn (#a : Type) (x : erased a) : tprop a
+  = {
+    t_hp  = Mem.emp;
+    t_sel = treturn_sel x;
+  }
+
+let treturn_int_sl (#a : Type) (x : erased a) (m : mem)
+  = Mem.intro_emp m
+
+let treturn_sel_eq (#a : Type) (x : erased a) (m : mem)
+  = ()
+
+let treturn_interp (#a : Type) (x : erased a)
+  = tprop_interp_intro _ _ _ _ _
+      (fun m _ -> Mem.intro_emp m) (fun m _ -> ()) (fun m0 m1 -> ()) (fun m0 m1 _ -> ())
+
+
+(***** [tbind] *)
+
+let tbind_vdep_rhs (#a #b : Type) (v : a -> tprop b) (x : a) : vprop
+  =
+    vprop_of_tprop (v x)
+
+let tbind_vprop (#a #b : Type) (u : tprop a) (v : a -> tprop b) : vprop
+  =
+    vrewrite (vprop_of_tprop u `vdep` tbind_vdep_rhs v) #b Mkdtuple2?._2
+
+let tbind (#a #b : Type) (u : tprop a) (v : a -> tprop b) : tprop b
+  =
+    tprop_of_vprop b (tbind_vprop u v)
+
+let tbind_int_sl (#a #b : Type) (u : tprop a) (v : a -> tprop b) (m : mem)
+  = interp_vdep_hp (vprop_of_tprop u) (tbind_vdep_rhs v) m
+
+let tbind_sel_eq (#a #b : Type) (u : tprop a) (v : a -> tprop b) (m : Mem.hmem (tbind u v).t_hp)
+  = tbind_int_sl u v m;
+    vrewrite_sel_eq (vprop_of_tprop u `vdep` tbind_vdep_rhs v) #b Mkdtuple2?._2 m;
+    vdep_sel_eq (vprop_of_tprop u) (tbind_vdep_rhs v) m
+
+let tbind_interp
+      #a #b u v
+      #u_guard #u_req #u_slp #u_sel u_tpi
+      #v_guard #v_req #v_slp #v_sel v_tpi
+  = tprop_interp_intro _ _ _ _ _
+    begin fun m _ ->
+      introduce interp (tbind u v).t_hp m ==> u_req m /\ v_req (u_sel m) m
+        with _ . (tbind_int_sl u v m; tprop_interp_elim u_tpi m; tprop_interp_elim (v_tpi (u_sel m)) m);
+      introduce u_req m /\ v_req (u_sel m) m ==>
+                (interp (tbind u v).t_hp m <==>
+                  (v_req (u_sel m) m /\ interp_opt (u_slp m `star_opt` v_slp (u_sel m) m) m))
+        with _ . begin
+        let x = u_sel m in
+        assert (u_guard m /\ (u_req m ==> v_guard x m));
+        calc (<==>) {
+          interp (tbind u v).t_hp m;
+        <==> { tbind_int_sl u v m }
+          interp u.t_hp m /\ interp (u.t_hp `Mem.star` (v (u.t_sel m)).t_hp) m;
+        <==> { tprop_interp_elim u_tpi m }
+          interp (u.t_hp `Mem.star` (v x).t_hp) m;
+        <==> { interp_star u.t_hp (v x).t_hp m }
+          exists (m0 m1 : mem) .
+            disjoint m0 m1 /\ join m0 m1 == m /\ interp u.t_hp m0 /\ interp (v x).t_hp m1;
+        <==> { let lem (m0 m1 : mem)
+               : Lemma (requires disjoint m0 m1 /\ join m0 m1 == m)
+                       (ensures  (interp u.t_hp     m0 <==> interp_opt (u_slp m)   m0) /\
+                                 (interp (v x).t_hp m1 <==> interp_opt (v_slp x m) m1))
+                       [SMTPat (disjoint m0 m1)]
+               =
+                 introduce (interp u.t_hp m0 \/ interp_opt (u_slp m) m0) ==>
+                           (interp u.t_hp m0 /\ interp_opt (u_slp m) m0)
+                   with _ . begin
+                     tprop_interp_join1 u_tpi m0 m1;
+                     tprop_interp_elim  u_tpi m0;
+                     tprop_interp_join0 u_tpi m0 m1
+                   end;
+                 introduce (interp (v x).t_hp m1 \/ interp_opt (v_slp x m) m1) ==>
+                           (interp (v x).t_hp m1 /\ interp_opt (v_slp x m) m1)
+                   with _ . begin
+                     Mem.join_commutative m0 m1;
+                     tprop_interp_join1 (v_tpi x) m1 m0;
+                     tprop_interp_elim  (v_tpi x) m1;
+                     tprop_interp_join0 (v_tpi x) m1 m0
+                   end
+             in ()
+           }
+          exists (m0 m1 : mem) .
+            disjoint m0 m1 /\ join m0 m1 == m /\ interp_opt (u_slp m) m0 /\ interp_opt (v_slp x m) m1;
+        <==> { interp_star_opt (u_slp m) (v_slp x m) m }
+          interp_opt (u_slp m `star_opt` v_slp x m) m;
+        }
+        end
+    end
+    begin fun m _ ->
+      tbind_int_sl u v m;
+      tbind_sel_eq u v m;
+      let x = u_sel m in
+      tprop_interp_elim u_tpi m;
+      calc (==) {
+        (tbind u v).t_sel m;
+      == { }
+        (v (u.t_sel m)).t_sel m;
+      == { }
+        (v x).t_sel m;
+      == { tprop_interp_elim (v_tpi x) m }
+        v_sel x m;
+      }
+    end
+    begin fun m0 m1 ->
+      let m = join m0 m1 in
+      assert (u_req m0 /\ v_req (u_sel m0) m0);
+      tprop_interp_join0 u_tpi m0 m1;
+      assert (u_req m /\ v_req (u_sel m) m0);
+      tprop_interp_join0 (v_tpi (u_sel m)) m0 m1;
+      assert (u_req m /\ v_req (u_sel m) m)
+    end
+    begin fun m0 m1 _ ->
+      let m = join m0 m1 in
+      let x = u_sel m    in
+      assert (u_guard m /\ u_req m /\ v_guard x m /\ v_req x m);
+      introduce interp (tbind u v).t_hp m0 ==> (interp u.t_hp m0 /\ interp (v x).t_hp m0)
+        with _ . begin
+          tbind_int_sl u v m0;
+          tprop_interp_elim u_tpi m
+        end;
+      assert ((interp      u.t_hp   m0 /\ interp     (v x).t_hp  m0) \/
+              (interp_opt (u_slp m) m0 /\ interp_opt (v_slp x m) m0));
+      tprop_interp_join1  u_tpi    m0 m1;
+      tprop_interp_join1 (v_tpi x) m0 m1;
+      assert (u_req m0 /\ v_req x m0);
+      tprop_interp_join0 u_tpi m0 m1;
+      assert (u_req m0 /\ v_req (u_sel m0) m0)
+    end
+
+
+(***** [tpure] *)
+
+let tpure_sel (p : Type0) : selector (squash p) (Mem.pure (p /\ True))
+  =
+    let sel' (m : Mem.hmem (Mem.pure (p /\ True))) : squash p = Mem.pure_interp (p /\ True) m in
+    sel'
+
+let tpure (p : Type0) : tprop (squash p)
+  = {
+    t_hp  = Mem.pure (p /\ True);
+    t_sel = tpure_sel p
+  }
+
+let tpure_int_sl (p : Type0) (m : mem)
+  = Mem.pure_interp (p /\ True) m
+
+let tpure_sel_eq (p : Type0) (m : Mem.hmem (tpure p).t_hp)
+  = tpure_int_sl p m
+
+let tpure_interp (p : Type0)
+  = tprop_interp_intro _ _ _ _ _
+      (fun m _ -> tpure_int_sl p m) (fun m _ -> ()) (fun m0 m1 -> ()) (fun m0 m1 _ -> ())
+
+
+(***** if-then-else *)
+
+let ite_interp_then
+      #a b thn els
+      #guard #req #slp #sel tpi
+  = tprop_interp_intro _ _ _ _ _
+      (fun m _ -> tpi.tpi_int_sl) (fun m _ -> tpi.tpi_sel_eq) (fun m0 m1 -> tpi.tpi_join0) (fun m0 m1 _ -> tpi.tpi_join1)
+
+let ite_interp_else
+      #a b thn els
+      #guard #req #slp #sel tpi
+  = tprop_interp_intro _ _ _ _ _
+      (fun m _ -> tpi.tpi_int_sl) (fun m _ -> tpi.tpi_sel_eq) (fun m0 m1 -> tpi.tpi_join0) (fun m0 m1 _ -> tpi.tpi_join1)
