steel/Learn.Steel.TProp.fsti
@@ -1,0 +1,307 @@
+module Learn.Steel.TProp
+
+module Mem = Steel.Memory
+open FStar.Ghost
+open Steel.Memory
+open Steel.Effect.Atomic
+
+
+(*** [tprop] *)
+
+[@@ erasable]
+noeq
+type tprop (t : Type0) = {
+  t_hp  : slprop u#1;
+  t_sel : selector t t_hp;
+}
+
+let tprop_of_vprop (t : Type) (v : vprop {normal (t_of v) == t}) : tprop t = {
+  t_hp  = hp_of v;
+  t_sel = sel_of v;
+}
+
+let vprop'_of_tprop (#t : Type) (u : tprop t) : vprop' = {
+  hp  = u.t_hp;
+  t;
+  sel = u.t_sel
+}
+
+let vprop_of_tprop (#t : Type) (u : tprop t) : vprop
+  = VUnit (vprop'_of_tprop u)
+
+
+(***** [tprop_interp] *)
+
+/// We use [option slprop] to avoid introducing some [Mem.emp] in the [slprop].
+
+let slprop_of_opt (slp : option slprop) : slprop
+  = match slp with
+  | Some slp -> slp
+  | None     -> Mem.emp
+
+let interp_opt (slp : option slprop) (m : mem) : prop
+  = match slp with
+  | Some slp -> interp slp m
+  | None     -> True
+
+val interp_of_opt (slp : option slprop) (m : mem)
+  : Lemma (interp_opt slp m <==> interp (slprop_of_opt slp) m)
+
+let star_opt (slp0 slp1 : option slprop) : option slprop
+  = match slp0 with
+    | None      -> slp1
+    | Some slp0 ->
+    match slp1 with
+    | None      -> Some slp0
+    | Some slp1 -> Some (slp0 `Mem.star` slp1)
+
+val star_of_opt (slp0 slp1 : option slprop)
+  : Lemma (slprop_of_opt (star_opt slp0 slp1) `Mem.equiv` (slprop_of_opt slp0 `Mem.star` slprop_of_opt slp1))
+
+val interp_star_opt (slp0 slp1 : option slprop) (m : mem)
+  : Lemma (interp_opt (star_opt slp0 slp1) m <==>
+            (exists (m0 m1 : mem) . disjoint m0 m1 /\ join m0 m1 == m /\ interp_opt slp0 m0 /\ interp_opt slp1 m1))
+
+
+type tprop_interp
+       (#t : Type) (u : tprop t)
+       (guard : (m : mem) -> prop)
+       (req   : (m : mem {guard m}) -> Type0)
+       (slp   : (m : mem {guard m /\ req m}) -> GTot (option slprop))
+       (sel   : (m : mem {guard m /\ req m}) -> GTot t)
+  = {
+    tpi_int_sl : squash (forall (m : mem {guard m}) . (interp u.t_hp m <==> req m /\ interp_opt (slp m) m));
+    tpi_sel_eq : squash (forall (m : Mem.hmem u.t_hp {guard m /\ req m}) . u.t_sel m == sel m);
+    tpi_join0  : squash (forall (m0: mem{guard m0 /\ req m0}) (m1:mem{disjoint m0 m1}) .
+                           guard (join m0 m1) /\ req (join m0 m1) /\
+                           slp (join m0 m1) == slp m0 /\ sel (join m0 m1) == sel m0);
+    tpi_join1  : squash (forall (m0:mem) (m1:mem{disjoint m0 m1}) .
+                           (guard (join m0 m1) /\ req (join m0 m1) /\
+                             (interp u.t_hp m0 \/ interp_opt (slp (join m0 m1)) m0)) ==>
+                           (guard m0 /\ req m0))
+  }
+
+val tprop_interp_intro
+      (#t : Type) (u : tprop t)
+      (guard : (m : mem) -> prop)
+      (req   : (m : mem {guard m}) -> Type0)
+      (slp   : (m : mem {guard m /\ req m}) -> GTot (option slprop))
+      (sel   : (m : mem {guard m /\ req m}) -> GTot t)
+      (int_sl : (m : mem) -> squash (guard m) ->
+                squash (interp u.t_hp m <==> req m /\ interp_opt (slp m) m))
+      (sel_eq : (m : Mem.hmem u.t_hp) -> squash (guard m /\ req m /\ interp_opt (slp m) m) ->
+                squash (u.t_sel m == sel m))
+      (join0  : (m0:mem{guard m0 /\ req m0}) -> (m1:mem{disjoint m0 m1}) ->
+                   squash (let m = join m0 m1 in guard m /\ req m /\ slp m == slp m0 /\ sel m == sel m0))
+      (join1  : (m0:mem) -> (m1:mem{disjoint m0 m1}) ->
+                   squash (let m = join m0 m1 in guard m /\ req m /\ (interp u.t_hp m0 \/ interp_opt (slp m) m0)) ->
+                   squash (guard m0 /\ req m0))
+  : tprop_interp u guard req slp sel
+
+val tprop_interp_elim
+      (#t : Type) (#u : tprop t)
+      (#guard : (m : mem) -> prop)
+      (#req   : (m : mem {guard m}) -> Type0)
+      (#slp   : (m : mem {guard m /\ req m}) -> GTot (option slprop))
+      (#sel   : (m : mem {guard m /\ req m}) -> GTot t)
+      (tpi    : tprop_interp u guard req slp sel)
+      (m : mem)
+  : Lemma (requires guard m)
+          (ensures (interp u.t_hp m <==> (req m /\ interp_opt (slp m) m)) /\
+                   (interp u.t_hp m ==> u.t_sel m == sel m))
+
+
+val tprop_trivial_interp (#t : Type) (u : tprop t)
+  : tprop_interp u (fun _ -> True) (interp (u.t_hp)) (fun _ -> Some u.t_hp) (u.t_sel)
+
+val tprop_of_vprop_interp (t : Type) (v : vprop {normal (t_of v) == t})
+  : tprop_interp (tprop_of_vprop t v) (fun _ -> True) (interp (hp_of v)) (fun _ -> Some (hp_of v)) (sel_of v)
+
+
+(*** Combinators *)
+
+// similar to the library of examples/steel/CQueue
+
+(***** [treturn] *)
+
+val treturn (#a : Type) (x : erased a) : tprop a
+
+val treturn_int_sl (#a : Type) (x : erased a) (m : mem)
+  : Lemma (interp (treturn x).t_hp m)
+
+val treturn_sel_eq (#a : Type) (x : erased a) (m : mem)
+  : Lemma (treturn_int_sl x m;
+           (treturn x).t_sel m == reveal x)
+
+val treturn_interp (#a : Type) (x : erased a)
+  : tprop_interp (treturn x) (fun _ -> True) (fun _ -> True) (fun _ -> None) (fun _ -> x)
+
+(***** [tbind] *)
+
+val tbind (#a #b : Type) (u : tprop a) (v : a -> tprop b) : tprop b
+
+val tbind_int_sl (#a #b : Type) (u : tprop a) (v : a -> tprop b) (m : mem)
+  : Lemma (interp (tbind u v).t_hp m <==>
+            (interp u.t_hp m /\ interp (u.t_hp `Mem.star` (v (u.t_sel m)).t_hp) m))
+
+val tbind_sel_eq (#a #b : Type) (u : tprop a) (v : a -> tprop b) (m : Mem.hmem (tbind u v).t_hp)
+  : Lemma (tbind_int_sl u v m;
+           (tbind u v).t_sel m == (v (u.t_sel m)).t_sel m)
+
+val tbind_interp
+      (#a #b : Type) (u : tprop a) (v : a -> tprop b)
+
+      (#u_guard : (m : mem) -> prop)
+      (#u_req   : (m : mem {u_guard m}) -> Type0)
+      (#u_slp   : (m : mem {u_guard m /\ u_req m}) -> GTot (option slprop))
+      (#u_sel   : (m : mem {u_guard m /\ u_req m}) -> GTot a)
+      (u_tpi    : tprop_interp u u_guard u_req u_slp u_sel)
+
+      (#v_guard : a -> (m : mem) -> prop)
+      (#v_req   : (x: a) -> (m : mem {v_guard x m}) -> Type0)
+      (#v_slp   : (x: a) -> (m : mem {v_guard x m /\ v_req x m}) -> GTot (option slprop))
+      (#v_sel   : (x: a) -> (m : mem {v_guard x m /\ v_req x m}) -> GTot b)
+      (v_tpi    : (x: a) -> tprop_interp (v x) (v_guard x) (v_req x) (v_slp x) (v_sel x))
+
+  : tprop_interp (tbind u v)
+      (fun m -> u_guard m /\ (u_req m ==> v_guard (u_sel m) m))
+      (fun m -> u_req m /\ v_req (u_sel m) m)
+      (fun m -> u_slp m `star_opt` v_slp (u_sel m) m)
+      (fun m -> v_sel (u_sel m) m)
+
+(***** [tpure] *)
+
+val tpure (p : Type0) : tprop (squash p)
+
+val tpure_int_sl (p : Type0) (m : mem)
+  : Lemma (interp (tpure p).t_hp m <==> p)
+
+val tpure_sel_eq (p : Type0) (m : Mem.hmem (tpure p).t_hp)
+  : Lemma (tpure_int_sl p m;
+           (tpure p).t_sel m == ())
+
+val tpure_interp (p : Type0)
+  : tprop_interp (tpure p) (fun _ -> True) (fun _ -> p) (fun _ -> None) (fun _ -> ())
+
+(***** if-then-else *)
+
+// ALT? explore both branches at the same time, remove guard
+
+val ite_interp_then
+      (#a : Type) (b : bool) (thn : tprop a) (els : tprop a)
+      (#guard : (m : mem) -> prop)
+      (#req   : (m : mem {guard m}) -> Type0)
+      (#slp   : (m : mem {guard m /\ req m}) -> GTot (option slprop))
+      (#sel   : (m : mem {guard m /\ req m}) -> GTot a)
+      (tpi    : tprop_interp thn guard req slp sel)
+  : tprop_interp (if b then thn else els) (fun m -> b /\ guard m) req slp sel
+
+val ite_interp_else
+      (#a : Type) (b : bool) (thn : tprop a) (els : tprop a)
+      (#guard : (m : mem) -> prop)
+      (#req   : (m : mem {guard m}) -> Type0)
+      (#slp   : (m : mem {guard m /\ req m}) -> GTot (option slprop))
+      (#sel   : (m : mem {guard m /\ req m}) -> GTot a)
+      (tpi    : tprop_interp els guard req slp sel)
+  : tprop_interp (if b then thn else els) (fun m -> ~b /\ guard m) req slp sel
+
+
+(*** Tactic *)
+
+module L = FStar.List.Pure
+open FStar.Tactics
+
+irreducible let __norm_tprop__ : unit = ()
+
+/// Solves a goal [tprop_interp #a tp ?guard ?req ?slp ?sel]
+let rec build_tprop_interp (branch : list int) : Tac (list int)
+  =
+    let goal = cur_goal () in
+    let _, args = collect_app goal in
+    guard (L.length args = 6);
+    let tp = (L.index args 1)._1 in
+    match inspect tp with
+    | Tv_App _ _ ->
+        let hd = match inspect (collect_app tp)._1 with
+                 | Tv_FVar v | Tv_UInst v _ -> v
+                 | _ -> fail "build_tprop_interp"
+        in let hd = implode_qn (inspect_fv hd) in
+        if hd = `%tprop_of_vprop
+        then (apply (`tprop_of_vprop_interp); branch)
+        else if hd = `%treturn
+        then (apply (`treturn_interp); branch)
+        else if hd = `%tbind
+        then begin
+          apply (`tbind_interp);
+          // u_tpi
+          let branch = build_tprop_interp branch in
+          // v_tpi
+          let x = intro () in
+          build_tprop_interp branch
+        end else if hd = `%tpure
+        then (apply (`tpure_interp); branch)
+        else fail "build_tprop_interp"
+    | Tv_Match _ _ _ -> // must be an if
+        begin match branch with
+        | 0 :: branch -> apply (`tprop_trivial_interp); branch
+        | 1 :: branch -> apply (`ite_interp_then);
+                       // We renormalize since the if was blocking the reduction
+                       norm [delta_attr [`%__norm_tprop__]];
+                       build_tprop_interp branch
+        | 2 :: branch -> apply (`ite_interp_else);
+                       norm [delta_attr [`%__norm_tprop__]];
+                       build_tprop_interp branch
+        | i :: branch -> fail ("invalid branch number: "^string_of_int i)
+        | []         -> fail "out of branches"
+        end
+    | _ -> fail "build_tprop_interp"
+
+private
+let __pose_interp_lemma
+      (#a : Type) (u : tprop a) (m : mem)
+      (#guard : (m : mem) -> prop)
+      (#req   : (m : mem {guard m}) -> Type0)
+      (#slp   : (m : mem {guard m /\ req m}) -> GTot (option slprop))
+      (#sel   : (m : mem {guard m /\ req m}) -> GTot a)
+      (tpi    : tprop_interp u guard req slp sel)
+      (hguard : squash (guard m))
+      (#goal  : Type)
+      (k      : squash ((interp u.t_hp m <==> req m /\ interp_opt (slp m) m) /\
+                        (interp u.t_hp m ==> u.t_sel m == sel m)) ->
+                goal)
+  : goal
+  = tprop_interp_elim tpi m;
+    k ()
+
+let pose_interp_lemma
+      (u : term) (m : term)
+      (rew_u : unit -> Tac unit)
+      (branch : list int) : Tac binder
+  =
+    apply (`__pose_interp_lemma (`#u) (`#m));
+    // tpi
+    rew_u ();
+    norm [delta_attr [`%__norm_tprop__]];
+    let branch = build_tprop_interp branch in
+    if Cons? branch then fail "remaining branches";
+    // hguard
+    norm [simplify]; smt ();
+    // k
+    let h = intro () in
+    norm_binder_type [delta_only [`%interp_opt; `%star_opt]; iota; zeta; simplify] h;
+    h
+
+
+(*** Notations *)
+
+/// Warning:
+/// The types inferred by F* for [bind] are often different from the types expected by the tactic.
+/// This lead to a `could not instantiate error`. When this happen, using [vprt] instead of [vpr] or
+/// adding an explicit type annotation on [return] (using the first, implicit, argument) can solve the problem.
+
+[@@__norm_tprop__] let return = treturn
+[@@__norm_tprop__] let bind (#a #b : Type) ($u : tprop a) (v : a -> tprop b) = tbind u v
+[@@__norm_tprop__] let vprt = tprop_of_vprop
+[@@__norm_tprop__] let vpr (v : vprop) = tprop_of_vprop (normal (t_of v)) v
+/// [tpr] should be used on [tprop] that are not unfolded (typically on recursive calls).
+[@@__norm_tprop__] let tpr (#a : Type) (t : tprop a) : tprop a = tprop_of_vprop a (vprop_of_tprop t)
